Finished proof of soundness without axiomatic fullness

theories/Core/Soundness/Extension/SystemAnnotated.v
@@ -3,89 +3,184 @@ From Coq Require Import List Classes.RelationClasses Setoid Morphisms.
 From McPTS Require Import PtsSignature LibTactics.
 From McPTS.Core Require Import Base.
 From McPTS.Core.Syntactic Require Export Syntax System Corollaries.
+From McPTS.Core.Soundness Require Import LogicalRelation.
 Import Syntax_Notations.
 
 
 Reserved Notation "⊫ Γ" (in custom judg at level 80, Γ custom exp).
-Reserved Notation "Γ ⊫ M : A > s" (in custom judg at level 80, Γ custom exp, M custom exp, A custom exp, s custom exp).
-Reserved Notation "Γ ⊫ A > s" (in custom judg at level 80, Γ custom exp, A custom exp, s custom exp).
+Reserved Notation "Γ ⊫ M : A @ s" (in custom judg at level 80, Γ custom exp, M custom exp, A custom exp, s custom exp).
+Reserved Notation "Γ ⊫ A @ s" (in custom judg at level 80, Γ custom exp, A custom exp, s custom exp).
 Reserved Notation "Γ ⊫s σ : Δ" (in custom judg at level 80, Γ custom exp, σ custom exp, Δ custom exp).
 
 Generalizable All Variables.
+
+(* Inductive wf_ctx_ann {P} : ctx P -> Prop := *)
+(* | wfa_ctx_empty : {{ ⊫ ⋅ }} *)
+(* | wfa_ctx_enxtend : *)
+(*   `( {{ ⊫ Γ }} -> *)
+(*      {{ Γ ⊫ A : Sort@s @ s' }} -> *)
+(*      {{ ⊫ Γ, A@s }} ) *)
+(* where "⊫ Γ" := (wf_ctx_ann Γ) (in custom judg) : type_scope *)
+(* with wf_exp_ann {P} : ctx P -> typ P -> P -> exp P -> Prop := *)
+(* (** Sorts *) *)
+(* | wfa_st : *)
+(*   `( Ax P s1 s2 -> Ax P s2 s3 -> *)
+(*      {{ ⊫ Γ }} -> *)
+(*      {{ Γ ⊫ Sort@s1 : Sort@s2 @ s3 }} ) *)
+
+(* (** Functions *) *)
+(* | wfa_pi : *)
+(*   `( forall (r : Ru P s1 s2 s3), *)
+(*         Ax P s3 s3' -> *)
+(*         {{ Γ ⊫ A : Sort@s1 @ s1' }} -> *)
+(*         {{ Γ, A@s1 ⊫ B : Sort@s2 @ s2' }} -> *)
+(*         {{ Γ ⊫ Π r A B : Sort@s3 @ s3' }} ) *)
+(* | wfa_fn : *)
+(*   `( forall (r : Ru P s1 s2 s3), *)
+(*         {{ Γ ⊫ A : Sort@s1 @ s1' }} -> *)
+(*         {{ Γ, A@s1 ⊫ B : Sort@s2 @ s2' }} -> *)
+(*         {{ Γ, A@s1 ⊫ M : B @ s2 }} -> *)
+(*         {{ Γ ⊫ λ r A M : Π r A B @ s3 }} ) *)
+(* | wfa_app : *)
+(*   `( forall (r : Ru P s1 s2 s3), *)
+(*         {{ Γ ⊫ A : Sort@s1 @ s1' }} -> *)
+(*         {{ Γ, A@s1 ⊫ B : Sort@s2 @ s2' }} -> *)
+(*         {{ Γ ⊫ M : Π r A B @ s3 }} -> *)
+(*         {{ Γ ⊫ N : A @ s1 }} -> *)
+(*         {{ Γ ⊫ M N : B[Id,,N] @ s2 }} ) *)
+
+(* (** Variables *) *)
+(* | wfa_vlookup : *)
+(*   `( {{ ⊫ Γ }} -> *)
+(*      {{ #x : A@s ∈ Γ }} -> *)
+(*      {{ Γ ⊫ #x : A @ s }} ) *)
+
+(* (** explicit substitutions *) *)
+(* | wfa_exp_sub_typ : *)
+(*   `( {{ Γ ⊫s σ : Δ }} -> *)
+(*      {{ Δ ⊫ M : A @ s }} -> *)
+(*      {{ Δ ⊫ A : Sort@s @ s' }} -> *)
+(*      {{ Γ ⊫ M[σ] : A[σ] @ s }} ) *)
+(* | wfa_exp_sub_sort : *)
+(*   `( {{ Γ ⊫s σ : Δ }} -> *)
+(*      {{ Δ ⊫ A : Sort@s @ s' }} -> *)
+(*      {{ Γ ⊫ A[σ] : Sort@s @ s' }} ) *)
+
+(* (** Conversions *) *)
+(* | wfa_exp_conv : *)
+(*   `( {{ Γ ⊫ M : A @ s }} -> *)
+(*      {{ Γ ⊫ A' : Sort@s @ s' }} -> *)
+(*      {{ Γ ⊢ A ≈ A' : Sort@s }} -> *)
+(*      {{ Γ ⊫ M : A' @ s }} ) *)
+(* | wfa_exp_conv_ann : *)
+(*   `( {{ Γ ⊫ M : A @ s }} -> *)
+(*      {{ Γ ⊫ A @ s' }} -> *)
+(*      {{ Γ ⊫ M : A @ s' }} ) *)
+(* where "Γ ⊫ M : A @ s" := (wf_exp_ann Γ A s M) (in custom judg) : type_scope *)
+
+(* with wf_typ_ann {P} : ctx P -> typ P -> P -> Prop := *)
+(* | wfa_typ_st : *)
+(*   `( Ax P s s' -> *)
+(*      {{ ⊫ Γ }} -> *)
+(*      {{ Γ ⊫ Sort@s @ s' }} ) *)
+(* | wfa_typ_exp : *)
+(*   `( {{ Γ ⊫ A : Sort@s @ s' }} -> *)
+(*      {{ Γ ⊫ A @ s }} ) *)
+(* where "Γ ⊫ A @ s" := (wf_typ_ann Γ A s) (in custom judg) : type_scope *)
+(* with wf_sub_ann {P} : ctx P -> ctx P -> sub P -> Prop := *)
+(* | wfa_sub_id : *)
+(*   `( {{ ⊫ Γ }} -> *)
+(*      {{ Γ ⊫s Id : Γ }} ) *)
+(* | wfa_sub_weaken : *)
+(*   `( {{ ⊫ Γ, A@s }} -> *)
+(*      {{ Γ, A@s ⊫s Wk : Γ }} ) *)
+(* | wfa_sub_compose : *)
+(*   `( {{ Γ1 ⊫s σ2 : Γ2 }} -> *)
+(*      {{ Γ2 ⊫s σ1 : Γ3 }} -> *)
+(*      {{ Γ1 ⊫s σ1∘σ2 : Γ3 }} ) *)
+(* | wfa_sub_extend : *)
+(*   `( {{ Γ ⊫s σ : Δ }} -> *)
+(*      {{ Δ ⊫ A : Sort@s @ s' }} -> *)
+(*      {{ Γ ⊫ M : A[σ] @ s }} -> *)
+(*      {{ Γ ⊫s σ,,M : Δ, A@s }} ) *)
+(* | wfa_sub_conv : *)
+(*   `( {{ Γ ⊫s σ : Δ }} -> *)
+(*      {{ ⊫ Δ' }} -> *)
+(*      {{ ⊢ Δ ≈ Δ' }} -> *)
+(*      {{ Γ ⊫s σ : Δ' }} ) *)
+(* where "Γ ⊫s σ : Δ" := (wf_sub_ann Γ Δ σ) (in custom judg) : type_scope. *)
 
 Inductive wf_ctx_ann {P} : ctx P -> Prop :=
 | wfa_ctx_empty : {{ ⊫ ⋅ }}
 | wfa_ctx_enxtend :
   `( {{ ⊫ Γ }} ->
-     {{ Γ ⊫ A : Sort@s > s' }} ->
+     {{ Γ ⊫ A : Sort@s @ s' }} ->
      {{ ⊫ Γ, A@s }} )
 where "⊫ Γ" := (wf_ctx_ann Γ) (in custom judg) : type_scope
-with wf_exp_ann {P} : ctx P -> typ P -> P -> exp P -> Prop :=
+with wf_exp_ann {P} : ctx P -> typ P -> SortOption P -> exp P -> Prop :=
 (** Sorts *)
 | wfa_st :
-  `( Ax P s1 s2 -> Ax P s2 s3 ->
+  `( Ax P s1 s2 ->
      {{ ⊫ Γ }} ->
-     {{ Γ ⊫ Sort@s1 : Sort@s2 > s3 }} )
+     {{ Γ ⊫ Sort@s1 : Sort@s2 @ ^None }} )
 
 (** Functions *)
 | wfa_pi :
   `( forall (r : Ru P s1 s2 s3),
-        Ax P s3 s3' ->
-        {{ Γ ⊫ A : Sort@s1 > s1' }} ->
-        {{ Γ, A@s1 ⊫ B : Sort@s2 > s2' }} ->
-        {{ Γ ⊫ Π r A B : Sort@s3 > s3' }} )
+        {{ Γ ⊫ A : Sort@s1 @ so1 }} ->
+        {{ Γ, A@s1 ⊫ B : Sort@s2 @ so2 }} ->
+        {{ Γ ⊫ Π r A B : Sort@s3 @ ^None }} )
 | wfa_fn :
   `( forall (r : Ru P s1 s2 s3),
-        {{ Γ ⊫ A : Sort@s1 > s1' }} ->
-        {{ Γ, A@s1 ⊫ B : Sort@s2 > s2' }} ->
-        {{ Γ, A@s1 ⊫ M : B > s2 }} ->
-        {{ Γ ⊫ λ r A M : Π r A B > s3 }} )
+        {{ Γ ⊫ A : Sort@s1 @ so1 }} ->
+        {{ Γ, A@s1 ⊫ B : Sort@s2 @ so2 }} ->
+        {{ Γ, A@s1 ⊫ M : B @ ^(Some s2) }} ->
+        {{ Γ ⊫ λ r A M : Π r A B @ ^(Some s3) }} )
 | wfa_app :
   `( forall (r : Ru P s1 s2 s3),
-        {{ Γ ⊫ A : Sort@s1 > s1' }} ->
-        {{ Γ, A@s1 ⊫ B : Sort@s2 > s2' }} ->
-        {{ Γ ⊫ M : Π r A B > s3 }} ->
-        {{ Γ ⊫ N : A > s1 }} ->
-        {{ Γ ⊫ M N : B[Id,,N] > s2 }} )
+        {{ Γ ⊫ A : Sort@s1 @ so1 }} ->
+        {{ Γ, A@s1 ⊫ B : Sort@s2 @ so2 }} ->
+        {{ Γ ⊫ M : Π r A B @ ^(Some s3) }} ->
+        {{ Γ ⊫ N : A @ ^(Some s1) }} ->
+        {{ Γ ⊫ M N : B[Id,,N] @ ^(Some s2) }} )
 
 (** Variables *)
 | wfa_vlookup :
   `( {{ ⊫ Γ }} ->
      {{ #x : A@s ∈ Γ }} ->
-     {{ Γ ⊫ #x : A > s }} )
+     {{ Γ ⊫ #x : A @ ^(Some s) }} )
 
 (** explicit substitutions *)
 | wfa_exp_sub_typ :
   `( {{ Γ ⊫s σ : Δ }} ->
-     {{ Δ ⊫ M : A > s }} ->
-     {{ Δ ⊫ A : Sort@s > s' }} ->
-     {{ Γ ⊫ M[σ] : A[σ] > s }} )
+     {{ Δ ⊫ M : A @ ^(Some s) }} ->
+     {{ Δ ⊫ A : Sort@s @ so }} ->
+     {{ Γ ⊫ M[σ] : A[σ] @ ^(Some s) }} )
 | wfa_exp_sub_sort :
   `( {{ Γ ⊫s σ : Δ }} ->
-     {{ Δ ⊫ A : Sort@s > s' }} ->
-     {{ Γ ⊫ A[σ] : Sort@s > s' }} )
+     {{ Δ ⊫ A : Sort@s @ so }} ->
+     {{ Γ ⊫ A[σ] : Sort@s @ so }} )
 
 (** Conversions *)
 | wfa_exp_conv :
-  `( {{ Γ ⊫ M : A > s }} ->
-     {{ Γ ⊫ A' : Sort@s > s' }} ->
+  `( {{ Γ ⊫ M : A @ ^(Some s) }} ->
+     {{ Γ ⊫ A' : Sort@s @ so }} ->
      {{ Γ ⊢ A ≈ A' : Sort@s }} ->
-     {{ Γ ⊫ M : A' > s }} )
+     {{ Γ ⊫ M : A' @ ^(Some s) }} )
 | wfa_exp_conv_ann :
-  `( {{ Γ ⊫ M : A > s }} ->
-     {{ Γ ⊫ A > s' }} ->
-     {{ Γ ⊫ M : A > s' }} )
-where "Γ ⊫ M : A > s" := (wf_exp_ann Γ A s M) (in custom judg) : type_scope
+  `( {{ Γ ⊫ M : A @ so }} ->
+     {{ Γ ⊫ A @ so' }} ->
+     {{ Γ ⊫ M : A @ so' }} )
+where "Γ ⊫ M : A @ s" := (wf_exp_ann Γ A s M) (in custom judg) : type_scope
 
-with wf_typ_ann {P} : ctx P -> typ P -> P -> Prop :=
+with wf_typ_ann {P} : ctx P -> typ P -> SortOption P -> Prop :=
 | wfa_typ_st :
-  `( Ax P s s' ->
-     {{ ⊫ Γ }} ->
-     {{ Γ ⊫ Sort@s > s' }} )
+  `( {{ ⊫ Γ }} ->
+     {{ Γ ⊫ Sort@s @ ^None }} )
 | wfa_typ_exp :
-  `( {{ Γ ⊫ A : Sort@s > s' }} ->
-     {{ Γ ⊫ A > s }} )
-where "Γ ⊫ A > s" := (wf_typ_ann Γ A s) (in custom judg) : type_scope
+  `( {{ Γ ⊫ A : Sort@s @ so }} ->
+     {{ Γ ⊫ A @ ^(Some s) }} )
+where "Γ ⊫ A @ s" := (wf_typ_ann Γ A s) (in custom judg) : type_scope
 with wf_sub_ann {P} : ctx P -> ctx P -> sub P -> Prop :=
 | wfa_sub_id :
   `( {{ ⊫ Γ }} ->
@@ -99,8 +194,8 @@ with wf_sub_ann {P} : ctx P -> ctx P -> sub P -> Prop :=
      {{ Γ1 ⊫s σ1∘σ2 : Γ3 }} )
 | wfa_sub_extend :
   `( {{ Γ ⊫s σ : Δ }} ->
-     {{ Δ ⊫ A : Sort@s > s' }} ->
-     {{ Γ ⊫ M : A[σ] > s }} ->
+     {{ Δ ⊫ A : Sort@s @ so }} ->
+     {{ Γ ⊫ M : A[σ] @ ^(Some s) }} ->
      {{ Γ ⊫s σ,,M : Δ, A@s }} )
 | wfa_sub_conv :
   `( {{ Γ ⊫s σ : Δ }} ->
@@ -108,6 +203,7 @@ with wf_sub_ann {P} : ctx P -> ctx P -> sub P -> Prop :=
      {{ ⊢ Δ ≈ Δ' }} ->
      {{ Γ ⊫s σ : Δ' }} )
 where "Γ ⊫s σ : Δ" := (wf_sub_ann Γ Δ σ) (in custom judg) : type_scope.
+
 
 #[export]
 Hint Constructors wf_ctx_ann wf_exp_ann wf_typ_ann wf_sub_ann : mcpts.
@@ -141,81 +237,125 @@ Ltac apply_fullness_all P full_P :=
 
 
 #[local]
-Ltac gen_annotated_judg_IH P full_P ann_ctx ann_exp ann_sub H :=
+Ltac gen_annotated_judg_IH P ann_ctx ann_exp ann_sub H :=
   match type of H with
   | {{ ⊢ ^?Γ }} =>
       let HΓ := fresh "HΓ" in
-      pose proof ann_ctx P full_P Γ H as HΓ
+      pose proof ann_ctx P Γ H as HΓ
   | {{ ^?Γ ⊢ ^?M : ^?A }} =>
       let HM := fresh "HM" in
-      pose proof ann_exp P full_P Γ M A H as HM
+      pose proof ann_exp P Γ M A H as HM
   | {{ ^?Γ ⊢s ^?σ : ^?Δ }} =>
       let Hσ := fresh "Hσ" in
-      pose proof ann_sub P full_P Γ σ Δ H as Hσ
+      pose proof ann_sub P Γ σ Δ H as Hσ
   end.
 
+#[local]
+Ltac gen_sort_none P :=
+  repeat
+    match goal with
+    | s : P |- _ =>
+        let Hs := fresh "Hs" in
+        eassert {{ ^?Γ ⊫ Sort@s @ ^None }} by mauto 3;
+        mark s
+    end;
+  unmark_all.
 
-
-
-Lemma wf_ctx_implies_wf_ctx_ann {P} (full_P : FullSig P) : forall {Γ : ctx P},
+ 
+Lemma wf_ctx_implies_wf_ctx_ann {P} : forall {Γ : ctx P},
     {{ ⊢ Γ }} -> {{ ⊫ Γ }}
-with wf_exp_implies_wf_exp_ann {P} (full_P : FullSig P) : forall {Γ : ctx P} {M A},
-    {{ Γ ⊢ M : A }} -> exists s, {{ Γ ⊫ M : A > s }}
-with wf_sub_implies_wf_sub_ann {P} (full_P : FullSig P) : forall {Γ : ctx P} {σ Δ},
+with wf_exp_implies_wf_exp_ann {P} : forall {Γ : ctx P} {M A},
+    {{ Γ ⊢ M : A }} -> exists so, {{ Γ ⊫ M : A @ so }}
+with wf_sub_implies_wf_sub_ann {P} : forall {Γ : ctx P} {σ Δ},
     {{ Γ ⊢s σ : Δ }} -> {{ Γ ⊫s σ : Δ }}.
 Proof.
   all: inversion_clear 1;
-    (on_all_hyp: gen_annotated_judg_IH P full_P wf_ctx_implies_wf_ctx_ann wf_exp_implies_wf_exp_ann wf_sub_implies_wf_sub_ann);
+    (on_all_hyp: gen_annotated_judg_IH P wf_ctx_implies_wf_ctx_ann wf_exp_implies_wf_exp_ann wf_sub_implies_wf_sub_ann);
     clear wf_ctx_implies_wf_ctx_ann wf_exp_implies_wf_exp_ann wf_sub_implies_wf_sub_ann;
     destruct_conjs;
-    apply_fullness_all P full_P;
     mauto 3.
 
   - eexists; econstructor; mauto 3.
-  - assert {{ Γ ⊫ Π r A0 B : Sort@s3 > s3' }} by mauto 3.
-    assert {{ Γ ⊫ Π r A0 B > s3 }} by mauto 3.
-    assert {{ Γ ⊫ M0 : Π r A0 B > s3 }} by mauto 2.
-    assert {{ Γ ⊫ A0 > s1 }} by mauto 2.
-    assert {{ Γ ⊫ N : A0 > s1 }} by mauto 2.
-    exists s2. mauto 3.
-  - assert {{ Δ ⊫ A0 > s }} by mauto 2.
-    assert {{ Δ ⊫ M0 : A0 > s }} by mauto 2.
-    eexists; econstructor; mauto 3.
-  - assert {{ Γ ⊫ M : A0 > s }} by mauto 3.
-    eexists; mauto 3.
-  - econstructor; mauto 3.
-    assert {{ Γ ⊫ A[σ0] : Sort@s > HM0 }} by mauto 3.
-    assert {{ Γ ⊫ A[σ0] > s }} by mauto 2.
+  - assert {{ Γ ⊫ Π r A0 B : Sort@s3 @ ^None }} by mauto 3.
+    assert {{ Γ ⊫ Π r A0 B @ ^(Some s3) }} by mauto 3.
+    assert {{ Γ ⊫ M0 : Π r A0 B @ ^(Some s3) }} by mauto 2.
+    assert {{ Γ ⊫ A0 @ ^(Some s1) }} by mauto 2.
+    assert {{ Γ ⊫ N : A0 @ ^(Some s1) }} by mauto 2.
+    eexists; mauto 2.
+  - assert {{ Δ ⊫ A0 @ ^(Some s) }} by mauto 2.
+    assert {{ Δ ⊫ M0 : A0 @ ^(Some s) }} by mauto 2.
+    eexists; mauto 2. 
+  - assert {{ Γ ⊫ M : A0 @ ^(Some s) }} by mauto 3.
+    eexists; mauto 2.
+  - assert {{ Γ ⊫ A[σ0] : Sort@s @ HM0 }} by mauto 3.
+    assert {{ Γ ⊫ A[σ0] @ ^(Some s) }} by mauto 2.
     mauto 3.
 Qed.
 
+#[export]
+Hint Resolve wf_ctx_implies_wf_ctx_ann wf_exp_implies_wf_exp_ann wf_sub_implies_wf_sub_ann : mcpts.
+ 
+(* Lemma wf_ctx_implies_wf_ctx_ann {P} (full_P : FullSig P) : forall {Γ : ctx P}, *)
+(*     {{ ⊢ Γ }} -> {{ ⊫ Γ }} *)
+(* with wf_exp_implies_wf_exp_ann {P} (full_P : FullSig P) : forall {Γ : ctx P} {M A}, *)
+(*     {{ Γ ⊢ M : A }} -> exists s, {{ Γ ⊫ M : A @ s }} *)
+(* with wf_sub_implies_wf_sub_ann {P} (full_P : FullSig P) : forall {Γ : ctx P} {σ Δ}, *)
+(*     {{ Γ ⊢s σ : Δ }} -> {{ Γ ⊫s σ : Δ }}. *)
+(* Proof. *)
+(*   all: inversion_clear 1; *)
+(*     (on_all_hyp: gen_annotated_judg_IH P full_P wf_ctx_implies_wf_ctx_ann wf_exp_implies_wf_exp_ann wf_sub_implies_wf_sub_ann); *)
+(*     clear wf_ctx_implies_wf_ctx_ann wf_exp_implies_wf_exp_ann wf_sub_implies_wf_sub_ann; *)
+(*     destruct_conjs; *)
+(*     apply_fullness_all P full_P; *)
+(*     mauto 3. *)
 
-Lemma wf_typ_full_implies_wf_exp {P} (full_P : FullSig P) : forall {Γ : ctx P} {A},
-    {{ Γ ⊢ A }} ->
-    exists s, {{ Γ ⊢ A : Sort@s }}.
-Proof.
-  inversion_clear 1; mauto 2.
-  assert (exists s', Ax P s s') as [s'] by (eapply full_P).
-  eexists; mauto 2.
-Qed.
+(*   - eexists; econstructor; mauto 3. *)
+(*   - assert {{ Γ ⊫ Π r A0 B : Sort@s3 @ s3' }} by mauto 3. *)
+(*     assert {{ Γ ⊫ Π r A0 B @ s3 }} by mauto 3. *)
+(*     assert {{ Γ ⊫ M0 : Π r A0 B @ s3 }} by mauto 2. *)
+(*     assert {{ Γ ⊫ A0 @ s1 }} by mauto 2. *)
+(*     assert {{ Γ ⊫ N : A0 @ s1 }} by mauto 2. *)
+(*     exists s2. mauto 3. *)
+(*   - assert {{ Δ ⊫ A0 @ s }} by mauto 2. *)
+(*     assert {{ Δ ⊫ M0 : A0 @ s }} by mauto 2. *)
+(*     eexists; econstructor; mauto 3. *)
+(*   - assert {{ Γ ⊫ M : A0 @ s }} by mauto 3. *)
+(*     eexists; mauto 3. *)
+(*   - econstructor; mauto 3. *)
+(*     assert {{ Γ ⊫ A[σ0] : Sort@s @ HM0 }} by mauto 3. *)
+(*     assert {{ Γ ⊫ A[σ0] @ s }} by mauto 2. *)
+(*     mauto 3. *)
+(* Qed. *)
 
 
-Lemma wf_typ_implies_wf_typ_ann {P} (full_P : FullSig P) : forall {Γ : ctx P} {A},
-    {{ Γ ⊢ A }} -> exists s, {{ Γ ⊫ A > s }}.
+(* Lemma wf_typ_full_implies_wf_exp {P} (full_P : FullSig P) : forall {Γ : ctx P} {A}, *)
+(*     {{ Γ ⊢ A }} -> *)
+(*     exists s, {{ Γ ⊢ A : Sort@s }}. *)
+(* Proof. *)
+(*   inversion_clear 1; mauto 2. *)
+(*   assert (exists s', Ax P s s') as [s'] by (eapply full_P). *)
+(*   eexists; mauto 2. *)
+(* Qed. *)
+
+
+Lemma wf_typ_implies_wf_typ_ann {P} : forall {Γ : ctx P} {A},
+    {{ Γ ⊢ A }} -> exists so, {{ Γ ⊫ A @ so }}.
 Proof.
   intros.
-  assert (exists s, {{ Γ ⊢ A : Sort@s }}) as [s] by (eapply wf_typ_full_implies_wf_exp; mauto 2).
-  eapply (wf_exp_implies_wf_exp_ann full_P) in H0.
-  destruct_conjs.
-  mauto 3.
+  destruct H.
+  - assert {{ ⊫ Γ }} by mauto 2.
+    eexists; mauto 2.
+  - assert (exists so, {{ Γ ⊫ A : Sort@s @ so }}) as [so] by mauto 2.
+    eexists; mauto 2.
 Qed.
 
-
+#[export]
+Hint Resolve wf_typ_implies_wf_typ_ann : mcpts.
 
 Lemma wf_judg_ann_implies_wf_judg {P} :
   (forall (Γ : ctx P), {{ ⊫ Γ }} -> {{ ⊢ Γ }}) /\
-    (forall (Γ : ctx P) A s M, {{ Γ ⊫ M : A > s }} -> {{ Γ ⊢ M : A }}) /\
-    (forall (Γ : ctx P) A s, {{ Γ ⊫ A > s }} -> {{ Γ ⊢ A }}) /\    
+    (forall (Γ : ctx P) A so M, {{ Γ ⊫ M : A @ so }} -> {{ Γ ⊢ M : A }}) /\
+    (forall (Γ : ctx P) A so, {{ Γ ⊫ A @ so }} -> {{ Γ ⊢ A }}) /\    
     (forall (Γ : ctx P) Δ σ, {{ Γ ⊫s σ : Δ }} -> {{ Γ ⊢s σ : Δ }}).
 Proof.
   eapply syntactic_wf_ann_mut_ind; mauto 2.
@@ -226,11 +366,11 @@ Corollary wf_ctx_ann_implies_wf_ctx {P} : forall {Γ : ctx P},
 Proof. intros; eapply wf_judg_ann_implies_wf_judg; mauto 2. Qed.
 
 Corollary wf_exp_ann_implies_wf_exp {P} : forall {Γ : ctx P} {A s M},
-    {{ Γ ⊫ M : A > s }} -> {{ Γ ⊢ M : A }}.
+    {{ Γ ⊫ M : A @ s }} -> {{ Γ ⊢ M : A }}.
 Proof. intros; eapply wf_judg_ann_implies_wf_judg; mauto 2. Qed.
 
 Corollary wf_typ_ann_implies_wf_typ {P} : forall {Γ : ctx P} {A s},
-    {{ Γ ⊫ A > s }} -> {{ Γ ⊢ A }}.
+    {{ Γ ⊫ A @ s }} -> {{ Γ ⊢ A }}.
 Proof. intros; eapply wf_judg_ann_implies_wf_judg; mauto 2. Qed.
 
 Corollary wf_sub_ann_implies_wf_sub {P} : forall {Γ : ctx P} {Δ σ},
