theories/Core/Soundness.v
@@ -7,59 +7,79 @@ From McPTS.Core.Soundness Require Export FundamentalTheorem.
 From McPTS.Core.Soundness.Extension Require Export SystemAnnotated.
 Import Domain_Notations.
 
-Theorem full_soundness {P} (pred_P : PredicativeSig P) (full_P : FullSig P) : forall {Γ : ctx P} {M A},
+Theorem soundness {P} (pred_P : PredicativeSig P) : forall {Γ : ctx P} {M A},
     {{ Γ ⊢ M : A }} ->
     exists W, nbe Γ M A W /\ {{ Γ ⊢ M ≈ W : A }}.
 Proof.
   intros * H.
   assert {{ ⊢ Γ }} by mauto 2.
   assert {{ ⟪ pred_P ⟫ ⊨ Γ }} as [env_relΓ] by (apply completeness_fundamental_ctx; eassumption).
-  destruct (soundness_fundamental_exp pred_P full_P _ _ _ H) as [s [Sb []]].
+  destruct (soundness_fundamental_exp pred_P _ _ _ H) as [so [Sb []]].
   pose proof (per_ctx_then_per_env_initial_env ltac:(eassumption)) as [p].
   destruct_conjs.
   functional_initial_env_rewrite_clear.
   assert {{ Γ ⊢s Id ® p ∈ Sb }} by (eapply initial_env_glu_rel_exp; mauto).
-  destruct_glu_rel_exp_with_sub.
-  assert {{ Γ ⊢ M[Id] : A[Id] ® m ∈ glu_elem_top pred_P s a }} as [] by (eapply realize_glu_elem_top; mauto).
-  match_by_head (@per_top P) ltac:(fun H => destruct (H (length Γ)) as [W []]).
-  eexists.
-  split; [econstructor |]; try eassumption.
-  assert {{ Γ ⊢ A[Id] ≈ A : Sort@s }} by mauto 3.
-  assert {{ Γ ⊢ A[Id][Id] ≈ A : Sort@s }} as HA by (transitivity {{{ A[Id] }}}; mauto 3).
-  assert {{ Γ ⊢ M[Id][Id] ≈ W : A[Id][Id] }} as HM by mauto 3.
-  assert {{ Γ ⊢ M[Id][Id] ≈ W : A }} as HM' by mauto 3.
-  assert {{ Γ ⊢ M[Id] ≈ M : A }} by mauto 3.
-  assert {{ Γ ⊢ M[Id][Id] ≈ M : A }} by (transitivity {{{ M[Id] }}}; mauto 3).
-  transitivity {{{ M[Id][Id] }}}; mauto 3.
+  destruct_glu_rel_exp_with_sub_unsorted.
+  -  assert {{ Γ ⊢ M[Id] : Sort@s ® m ∈ glu_elem_top_unsorted pred_P None d{{{ Sort@s }}} }} by (eapply realize_glu_elem_top_unsorted; mauto).
+    simpl in H6.
+    dependent destruction H6.
+    match_by_head (@per_top P) ltac:(fun H => destruct (H (length Γ)) as [W []]).
+    eexists.
+    split; [econstructor |]; try eassumption; [mauto 2|].
+    dependent destruction H10.
+    dependent destruction H12.
+    simpl_glu_rel.    
+    assert {{ Γ ⊢ M[Id][Id] ≈ W : Sort@s }} as HM by mauto 3.
+    assert {{ Γ ⊢ M[Id][Id] ≈ W : Sort@s }} as HM' by mauto 3.
+    assert {{ Γ ⊢ M[Id] ≈ M : Sort@s }} by mauto 3.
+    assert {{ Γ ⊢ M[Id][Id] ≈ M : Sort@s }} by (transitivity {{{ M[Id] }}}; mauto 3).
+    transitivity {{{ M[Id][Id] }}}; mauto 3.
+
+  - assert {{ Γ ⊢ M[Id] : A[Id] ® m ∈ glu_elem_top pred_P s a }} as [] by (eapply realize_glu_elem_top; mauto).
+    match_by_head (@per_top P) ltac:(fun H => destruct (H (length Γ)) as [W []]).
+    eexists.
+    split; [econstructor |]; try eassumption.
+    assert {{ Γ ⊢ A[Id] : Sort@s }} by (eapply glu_sort_elem_sort_lvl; mauto 2).
+    assert {{ Γ ⊢ A[Id] ≈ A : Sort@s }} by mauto 3.
+    assert {{ Γ ⊢ A[Id][Id] ≈ A : Sort@s }} as HA by (transitivity {{{ A[Id] }}}; mauto 3).
+    assert {{ Γ ⊢ M[Id][Id] ≈ W : A[Id][Id] }} as HM by mauto 3.
+    assert {{ Γ ⊢ M[Id][Id] ≈ W : A }} as HM' by mauto 3.
+    assert {{ Γ ⊢ M[Id] ≈ M : A }} by mauto 3.
+    assert {{ Γ ⊢ M[Id][Id] ≈ M : A }} by (transitivity {{{ M[Id] }}}; mauto 3).
+    transitivity {{{ M[Id][Id] }}}; mauto 3.
 Qed.
 
-Theorem full_soundness' {P} (pred_P : PredicativeSig P) (full_P : FullSig P) : forall {Γ : ctx P} {M A W},
+Theorem soundness' {P} (pred_P : PredicativeSig P) : forall {Γ : ctx P} {M A W},
     {{ Γ ⊢ M : A }} ->
     nbe Γ M A W ->
     {{ Γ ⊢ M ≈ W : A }}.
 Proof.
-  intros * [? []]%(full_soundness pred_P full_P) ?.
+  intros * [? []]%(soundness pred_P) ?.
   functional_nbe_rewrite_clear.
   eassumption.
 Qed.
 
-Lemma full_soundness_ty {P} (pred_P : PredicativeSig P) (full_P : FullSig P) : forall {Γ : ctx P} {A},
+Lemma soundness_ty {P} (pred_P : PredicativeSig P) : forall {Γ : ctx P} {A},
     {{ Γ ⊢ A }} ->
     exists W, nbe_ty Γ A W /\ {{ Γ ⊢ A ≈ W }}.
 Proof.
   intros.
-  assert (exists s, {{ Γ ⊢ A : Sort@s }}) as [s] by (eapply wf_typ_full_implies_wf_exp; mauto 2).
-  assert (exists W, nbe Γ A {{{ Sort@s }}} W /\ {{ Γ ⊢ A ≈ W : Sort@s }}) as [W [?%nbe_type_to_nbe_ty Heq]] by mauto using full_soundness.
-  eexists; split; mauto 3.
+  destruct H.
+  - assert {{ ⟪ pred_P ⟫ ⊨ Γ }} as [env_relΓ] by (eapply completeness_fundamental_ctx; mauto 2).
+    assert (exists p p', initial_env Γ p /\ initial_env Γ p' /\ {{ Dom p ≈ p' ∈ env_relΓ }}) as [p] by (eauto using per_ctx_then_per_env_initial_env).
+    destruct_conjs.
+    eexists; split; [econstructor|]; mauto 3.
+  - assert (exists W, nbe Γ A {{{ Sort@s }}} W /\ {{ Γ ⊢ A ≈ W : Sort@s }}) as [W [?%nbe_type_to_nbe_ty Heq]] by mauto using soundness.
+    eexists; split; mauto 3.
 Qed.
 
-Lemma full_soundness_ty' {P} (pred_P : PredicativeSig P) (full_P : FullSig P) : forall {Γ : ctx P} {A W},
+Lemma soundness_ty' {P} (pred_P : PredicativeSig P) : forall {Γ : ctx P} {A W},
     {{ Γ ⊢ A }} ->
     nbe_ty Γ A W ->
     {{ Γ ⊢ A ≈ W }}.
 Proof.
   intros.
-  assert (exists B', nbe_ty Γ A B' /\ {{ Γ ⊢ A ≈ B' }}) as [? [? Heq]] by mauto using full_soundness_ty.
+  assert (exists B', nbe_ty Γ A B' /\ {{ Γ ⊢ A ≈ B' }}) as [? [? Heq]] by mauto using soundness_ty.
   functional_nbe_rewrite_clear.
   eassumption.
 Qed.
