theories/Core/Soundness/FundamentalTheorem.v
@@ -11,58 +11,57 @@ From McPTS.Core.Soundness.Extension Require Import SystemAnnotated.
 Import Domain_Notations.
 
 Section soundness_fundamental.
-  Theorem soundness_fundamental {P} (pred_P : PredicativeSig P) (full_P : FullSig P) :
+  Theorem soundness_fundamental {P} (pred_P : PredicativeSig P) :
     (forall Γ, {{ ⊫ Γ }} -> {{ ⟪ pred_P ⟫ ⊩ Γ }}) /\
-      (forall Γ A s M, {{ Γ ⊫ M : A > s }} -> {{ ⟪ pred_P ⟫ Γ ⊩ M : A > s }}) /\
-      (forall Γ A s, {{ Γ ⊫ A > s }} -> {{ ⟪ pred_P ⟫ Γ ⊩ A > s }}) /\
+      (forall Γ A s M, {{ Γ ⊫ M : A @ s }} -> {{ ⟪ pred_P ⟫ Γ ⊩u M : A @ s }}) /\
+      (forall Γ A s, {{ Γ ⊫ A @ s }} -> {{ ⟪ pred_P ⟫ Γ ⊩u A @ s }}) /\
       (forall Γ Δ σ, {{ Γ ⊫s σ : Δ }} -> {{ ⟪ pred_P ⟫ Γ ⊩s σ : Δ }}).
   Proof.
     eapply syntactic_wf_ann_mut_ind; mauto 3; intros.
   Qed.
 
   #[local]
-  Ltac solve_it pred_P full_P := pose proof soundness_fundamental pred_P full_P; firstorder.
+  Ltac solve_it pred_P := pose proof soundness_fundamental pred_P; firstorder.
   
-  Corollary soundness_fundamental_ctx_ann {P} (pred_P : PredicativeSig P) (full_P : FullSig P) :
+  Corollary soundness_fundamental_ctx_ann {P} (pred_P : PredicativeSig P) :
     forall Γ, {{ ⊫ Γ }} -> {{ ⟪ pred_P ⟫ ⊩ Γ }}.
-  Proof. solve_it pred_P full_P. Qed.
+  Proof. solve_it pred_P. Qed.
   
-  Corollary soundness_fundamental_exp_ann {P} (pred_P : PredicativeSig P) (full_P : FullSig P) :
-    forall Γ A s M, {{ Γ ⊫ M : A > s }} -> {{ ⟪ pred_P ⟫ Γ ⊩ M : A > s }}.
-  Proof. solve_it pred_P full_P. Qed.
+  Corollary soundness_fundamental_exp_ann {P} (pred_P : PredicativeSig P) :
+    forall Γ A so M, {{ Γ ⊫ M : A @ so }} -> {{ ⟪ pred_P ⟫ Γ ⊩u M : A @ so }}.
+  Proof. solve_it pred_P. Qed.
   
-  Corollary soundness_fundamental_typ_ann {P} (pred_P : PredicativeSig P) (full_P : FullSig P) :
-    forall Γ A s, {{ Γ ⊫ A > s }} -> {{ ⟪ pred_P ⟫ Γ ⊩ A > s }}.
-  Proof. solve_it pred_P full_P. Qed.
+  Corollary soundness_fundamental_typ_ann {P} (pred_P : PredicativeSig P) :
+    forall Γ A so, {{ Γ ⊫ A @ so }} -> {{ ⟪ pred_P ⟫ Γ ⊩u A @ so }}.
+  Proof. solve_it pred_P. Qed.
   
-  Corollary soundness_fundamental_sub_ann {P} (pred_P : PredicativeSig P) (full_P : FullSig P) :
+  Corollary soundness_fundamental_sub_ann {P} (pred_P : PredicativeSig P) :
     forall Γ Δ σ, {{ Γ ⊫s σ : Δ }} -> {{ ⟪ pred_P ⟫ Γ ⊩s σ : Δ }}.
-  Proof. solve_it pred_P full_P. Qed.  
-
+  Proof. solve_it pred_P. Qed.  
 
   
-  Theorem soundness_fundamental_ctx {P} (pred_P : PredicativeSig P) (full_P : FullSig P) :
+  Theorem soundness_fundamental_ctx {P} (pred_P : PredicativeSig P) :
     forall Γ, {{ ⊢ Γ }} -> {{ ⟪ pred_P ⟫ ⊩ Γ }}.
   Proof.
     intros.
-    assert {{ ⊫ Γ }} by (eapply wf_ctx_implies_wf_ctx_ann; mauto 2).
+    assert {{ ⊫ Γ }} by mauto 2. 
     eapply soundness_fundamental_ctx_ann; mauto 2.
   Qed.
 
-  Theorem soundness_fundamental_exp {P} (pred_P : PredicativeSig P) (full_P : FullSig P) :
-    forall Γ M A, {{ Γ ⊢ M : A }} -> exists s, {{ ⟪ pred_P ⟫ Γ ⊩ M : A > s }}.
+  Theorem soundness_fundamental_exp {P} (pred_P : PredicativeSig P) :
+    forall Γ M A, {{ Γ ⊢ M : A }} -> exists so, {{ ⟪ pred_P ⟫ Γ ⊩u M : A @ so }}.
   Proof.
     intros.
-    assert (exists s, {{ Γ ⊫ M : A > s }}) as [s] by (eapply wf_exp_implies_wf_exp_ann; mauto 2).
+    assert (exists so, {{ Γ ⊫ M : A @ so }}) as [so] by mauto 2.
     eexists.
     eapply soundness_fundamental_exp_ann; mauto 2.
   Qed.
 
-  Theorem soundness_fundamental_typ {P} (pred_P : PredicativeSig P) (full_P : FullSig P) :
-    forall Γ A, {{ Γ ⊢ A }} -> exists s, {{ ⟪ pred_P ⟫ Γ ⊩ A > s }}.
+  Theorem soundness_fundamental_typ {P} (pred_P : PredicativeSig P) :
+    forall Γ A, {{ Γ ⊢ A }} -> exists so, {{ ⟪ pred_P ⟫ Γ ⊩u A @ so }}.
   Proof.
     intros.
-    assert (exists s, {{ Γ ⊫ A > s }}) as [s] by (eapply wf_typ_implies_wf_typ_ann; mauto 2).
+    assert (exists so, {{ Γ ⊫ A @ so }}) as [so] by mauto 2.
     eexists.
     eapply soundness_fundamental_typ_ann; mauto 2.
   Qed.
@@ -71,7 +70,76 @@ Section soundness_fundamental.
     forall Γ σ Δ, {{ Γ ⊢s σ : Δ }} -> {{ ⟪ pred_P ⟫ Γ ⊩s σ : Δ }}.
   Proof.
     intros.
-    assert {{ Γ ⊫s σ : Δ }} by (eapply wf_sub_implies_wf_sub_ann; mauto 2).
+    assert {{ Γ ⊫s σ : Δ }} by mauto 2.
     eapply soundness_fundamental_sub_ann; mauto 2.
   Qed.  
 End soundness_fundamental.
+
+
+
+
+(* Section soundness_fundamental. *)
+(*   Theorem soundness_fundamental {P} (pred_P : PredicativeSig P) (full_P : FullSig P) : *)
+(*     (forall Γ, {{ ⊫ Γ }} -> {{ ⟪ pred_P ⟫ ⊩ Γ }}) /\ *)
+(*       (forall Γ A s M, {{ Γ ⊫ M : A @ s }} -> {{ ⟪ pred_P ⟫ Γ ⊩ M : A @ s }}) /\ *)
+(*       (forall Γ A s, {{ Γ ⊫ A @ s }} -> {{ ⟪ pred_P ⟫ Γ ⊩ A @ s }}) /\ *)
+(*       (forall Γ Δ σ, {{ Γ ⊫s σ : Δ }} -> {{ ⟪ pred_P ⟫ Γ ⊩s σ : Δ }}). *)
+(*   Proof. *)
+(*     eapply syntactic_wf_ann_mut_ind; mauto 3; intros. *)
+(*   Qed. *)
+
+(*   #[local] *)
+(*   Ltac solve_it pred_P full_P := pose proof soundness_fundamental pred_P full_P; firstorder. *)
+  
+(*   Corollary soundness_fundamental_ctx_ann {P} (pred_P : PredicativeSig P) (full_P : FullSig P) : *)
+(*     forall Γ, {{ ⊫ Γ }} -> {{ ⟪ pred_P ⟫ ⊩ Γ }}. *)
+(*   Proof. solve_it pred_P full_P. Qed. *)
+  
+(*   Corollary soundness_fundamental_exp_ann {P} (pred_P : PredicativeSig P) (full_P : FullSig P) : *)
+(*     forall Γ A s M, {{ Γ ⊫ M : A @ s }} -> {{ ⟪ pred_P ⟫ Γ ⊩ M : A @ s }}. *)
+(*   Proof. solve_it pred_P full_P. Qed. *)
+  
+(*   Corollary soundness_fundamental_typ_ann {P} (pred_P : PredicativeSig P) (full_P : FullSig P) : *)
+(*     forall Γ A s, {{ Γ ⊫ A @ s }} -> {{ ⟪ pred_P ⟫ Γ ⊩ A @ s }}. *)
+(*   Proof. solve_it pred_P full_P. Qed. *)
+  
+(*   Corollary soundness_fundamental_sub_ann {P} (pred_P : PredicativeSig P) (full_P : FullSig P) : *)
+(*     forall Γ Δ σ, {{ Γ ⊫s σ : Δ }} -> {{ ⟪ pred_P ⟫ Γ ⊩s σ : Δ }}. *)
+(*   Proof. solve_it pred_P full_P. Qed.   *)
+
+
+  
+(*   Theorem soundness_fundamental_ctx {P} (pred_P : PredicativeSig P) (full_P : FullSig P) : *)
+(*     forall Γ, {{ ⊢ Γ }} -> {{ ⟪ pred_P ⟫ ⊩ Γ }}. *)
+(*   Proof. *)
+(*     intros. *)
+(*     assert {{ ⊫ Γ }} by (eapply wf_ctx_implies_wf_ctx_ann; mauto 2). *)
+(*     eapply soundness_fundamental_ctx_ann; mauto 2. *)
+(*   Qed. *)
+
+(*   Theorem soundness_fundamental_exp {P} (pred_P : PredicativeSig P) (full_P : FullSig P) : *)
+(*     forall Γ M A, {{ Γ ⊢ M : A }} -> exists s, {{ ⟪ pred_P ⟫ Γ ⊩ M : A @ s }}. *)
+(*   Proof. *)
+(*     intros. *)
+(*     assert (exists s, {{ Γ ⊫ M : A @ s }}) as [s] by (eapply wf_exp_implies_wf_exp_ann; mauto 2). *)
+(*     eexists. *)
+(*     eapply soundness_fundamental_exp_ann; mauto 2. *)
+(*   Qed. *)
+
+(*   Theorem soundness_fundamental_typ {P} (pred_P : PredicativeSig P) (full_P : FullSig P) : *)
+(*     forall Γ A, {{ Γ ⊢ A }} -> exists s, {{ ⟪ pred_P ⟫ Γ ⊩ A @ s }}. *)
+(*   Proof. *)
+(*     intros. *)
+(*     assert (exists s, {{ Γ ⊫ A @ s }}) as [s] by (eapply wf_typ_implies_wf_typ_ann; mauto 2). *)
+(*     eexists. *)
+(*     eapply soundness_fundamental_typ_ann; mauto 2. *)
+(*   Qed. *)
+  
+(*   Theorem soundness_fundamental_sub {P} (pred_P : PredicativeSig P) (full_P : FullSig P) : *)
+(*     forall Γ σ Δ, {{ Γ ⊢s σ : Δ }} -> {{ ⟪ pred_P ⟫ Γ ⊩s σ : Δ }}. *)
+(*   Proof. *)
+(*     intros. *)
+(*     assert {{ Γ ⊫s σ : Δ }} by (eapply wf_sub_implies_wf_sub_ann; mauto 2). *)
+(*     eapply soundness_fundamental_sub_ann; mauto 2. *)
+(*   Qed.   *)
+(* End soundness_fundamental. *)
